chore: add recursive rewriter, stuck at one case of the correctness proof

SSA/Core/Framework.lean
@@ -2463,6 +2463,91 @@ theorem denote_rewritePeephole (fuel : ℕ)
 /-- info: 'denote_rewritePeephole' depends on axioms: [propext, Classical.choice, Quot.sound] -/
 #guard_msgs in #print axioms denote_rewritePeephole
 
+mutual
+
+def rewritePeepholeRecursivelyHVectorCom (fuel : ℕ)
+    (pr : PeepholeRewrite d Γ t) {ts :  List (Ctxt d.Ty × d.Ty)}
+    (args : HVector (fun t => Com d t.1 EffectKind.impure t.2) ts)
+    : HVector (fun t => Com d t.1 EffectKind.impure t.2) ts :=
+  match h : ts with
+  | .nil =>
+    match args with
+    | .nil => HVector.nil
+  | .cons _ _ =>
+    match args with
+    | .cons com coms =>
+      .cons (rewritePeepholeRecursivelyCom fuel pr com) (rewritePeepholeRecursivelyHVectorCom fuel pr coms)
+
+def rewritePeepholeRecursivelyCom (fuel : ℕ)
+    (pr : PeepholeRewrite d Γ t) (target : Com d Γ₂ eff t₂) : Com d Γ₂ eff t₂ :=
+  match fuel with
+  | 0 => target
+  | fuel + 1 =>
+    let target := rewritePeephole fuel pr target
+    match target with
+    | .ret v => target
+    | .var e body =>
+      let e' :=
+        match e with
+        | Expr.mk op ty eff args regArgs =>
+          Expr.mk op ty eff args (rewritePeepholeRecursivelyHVectorCom fuel pr regArgs)
+      let body' :=
+        -- decreases because 'body' is smaller.
+        rewritePeepholeRecursivelyCom fuel pr body
+      .var e' body'
+end
+
+mutual
+theorem denote_rewritePeepholeRecursivelyHVectorCom (fuel : ℕ)
+    (pr : PeepholeRewrite d Γ t) {ts :  List (Ctxt d.Ty × d.Ty)}
+    (args : HVector (fun t => Com d t.1 EffectKind.impure t.2) ts)
+    : (rewritePeepholeRecursivelyHVectorCom fuel pr args).denote = args.denote := by
+  induction ts
+  case nil =>
+    simp [rewritePeepholeRecursivelyHVectorCom]
+  case cons ts' hts =>
+    simp [rewritePeepholeRecursivelyHVectorCom, denote_rewritePeepholeRecursivelyCom, hts]
+    cases args
+    case cons com coms =>
+      simp [rewritePeepholeRecursivelyHVectorCom, denote_rewritePeepholeRecursivelyCom, hts]
+
+
+theorem denote_rewritePeepholeRecursivelyCom (fuel : ℕ) (pr : PeepholeRewrite d Γ t) (target : Com d Γ₂ eff t₂) :
+    (rewritePeepholeRecursivelyCom fuel pr target).denote = target.denote := by
+  induction fuel generalizing target
+  case zero =>
+    simp [rewritePeepholeRecursivelyCom]
+  case succ fuel' hfuel =>
+    induction target generalizing Γ
+    case ret u v w ty effKind v =>
+      simp [rewritePeepholeRecursivelyCom]
+      cases htarget : rewritePeephole fuel' pr (Com.ret v)
+      case ret v' =>
+        have hdenote_eq : (rewritePeephole (eff := effKind) fuel' pr (Com.ret v)).denote = (Com.ret v).denote := by
+          apply denote_rewritePeephole
+        rw [htarget] at hdenote_eq
+        simp only [Com.denote_ret, EffectKind.return_impure_toMonad_eq] at hdenote_eq
+        simp [hdenote_eq]
+      case var e body =>
+        have hdenote_eq : (rewritePeephole (eff := effKind) fuel' pr (Com.ret v)).denote = (Com.ret v).denote := by
+          apply denote_rewritePeephole
+        rw [htarget] at hdenote_eq
+        simp at hdenote_eq
+        simp
+        rcases e with ⟨op, ty, eff, args, regArgs⟩
+        subst ty
+        funext Γv
+        simp_all [Expr.denote]
+        simp_all [rewritePeepholeRecursivelyHVectorCom, denote_rewritePeepholeRecursivelyHVectorCom]
+        simp [hfuel body]
+
+        -- this is true, because the denote of rewritePeephole equals
+        -- that of denotePeephole'
+        sorry
+    simp [rewritePeepholeRecursivelyCom, denote_rewritePeephole, hfuel, denote_rewritePeepholeRecursivelyHVectorCom]
+
+end
+
 end SimpPeepholeApplier
 
 section TypeProjections
